Translate UniqSet

examples/ghc/lib/UniqSet.v
@@ -22,30 +22,20 @@ Import GHC.Base.Notations.
 
 (* Converted type declarations: *)
 
-Inductive UniqSet a : Type := UniqSet : UniqFM.UniqFM a -> UniqSet a.
+Inductive UniqSet a : Type := Mk_UniqSet : UniqFM.UniqFM a -> UniqSet a.
 
-Arguments UniqSet {_} _.
+Arguments Mk_UniqSet {_} _.
 
 Definition getUniqSet' {a} (arg_0__ : UniqSet a) :=
-  let 'UniqSet getUniqSet' := arg_0__ in
+  let 'Mk_UniqSet getUniqSet' := arg_0__ in
   getUniqSet'.
 (* Converted value declarations: *)
 
-Local Definition Eq___UniqSet_op_zeze__ {inst_a}
-   : (UniqSet inst_a) -> (UniqSet inst_a) -> bool :=
-  fun arg_0__ arg_1__ =>
-    match arg_0__, arg_1__ with
-    | UniqSet a, UniqSet b => UniqFM.equalKeysUFM a b
-    end.
+Instance Unpeel_UniqSet ele
+   : GHC.Prim.Unpeel (UniqSet ele) (UniqFM.UniqFM ele) :=
+  GHC.Prim.Build_Unpeel _ _ (fun x => let 'Mk_UniqSet y := x in y) Mk_UniqSet.
 
-Local Definition Eq___UniqSet_op_zsze__ {inst_a}
-   : (UniqSet inst_a) -> (UniqSet inst_a) -> bool :=
-  fun x y => negb (Eq___UniqSet_op_zeze__ x y).
-
-Program Instance Eq___UniqSet {a} : GHC.Base.Eq_ (UniqSet a) :=
-  fun _ k =>
-    k {| GHC.Base.op_zeze____ := Eq___UniqSet_op_zeze__ ;
-         GHC.Base.op_zsze____ := Eq___UniqSet_op_zsze__ |}.
+(* Skipping instance Eq___UniqSet *)
 
 (* Translating `instance Outputable__UniqSet' failed: OOPS! Cannot find
    information for class Qualified "Outputable" "Outputable" unsupported *)
@@ -59,13 +49,7 @@ Local Definition Monoid__UniqSet_mconcat {inst_a}
   GHC.Prim.coerce GHC.Base.mconcat.
 
 Local Definition Monoid__UniqSet_mempty {inst_a} : UniqSet inst_a :=
-  GHC.Prim.coerce GHC.Base.mempty.
-
-Program Instance Monoid__UniqSet {a} : GHC.Base.Monoid (UniqSet a) :=
-  fun _ k =>
-    k {| GHC.Base.mappend__ := Monoid__UniqSet_mappend ;
-         GHC.Base.mconcat__ := Monoid__UniqSet_mconcat ;
-         GHC.Base.mempty__ := Monoid__UniqSet_mempty |}.
+  Mk_UniqSet GHC.Base.mempty.
 
 Local Definition Semigroup__UniqSet_op_zlzlzgzg__ {inst_a}
    : UniqSet inst_a -> UniqSet inst_a -> UniqSet inst_a :=
@@ -74,6 +58,12 @@ Local Definition Semigroup__UniqSet_op_zlzlzgzg__ {inst_a}
 Program Instance Semigroup__UniqSet {a} : GHC.Base.Semigroup (UniqSet a) :=
   fun _ k => k {| GHC.Base.op_zlzlzgzg____ := Semigroup__UniqSet_op_zlzlzgzg__ |}.
 
+Program Instance Monoid__UniqSet {a} : GHC.Base.Monoid (UniqSet a) :=
+  fun _ k =>
+    k {| GHC.Base.mappend__ := Monoid__UniqSet_mappend ;
+         GHC.Base.mconcat__ := Monoid__UniqSet_mconcat ;
+         GHC.Base.mempty__ := Monoid__UniqSet_mempty |}.
+
 (* Translating `instance Data__UniqSet' failed: OOPS! Cannot find information
    for class Qualified "Data.Data" "Data" unsupported *)
 
@@ -81,7 +71,7 @@ Definition addOneToUniqSet {a} `{Unique.Uniquable a}
    : UniqSet a -> a -> UniqSet a :=
   fun arg_0__ arg_1__ =>
     match arg_0__, arg_1__ with
-    | UniqSet set, x => UniqSet (UniqFM.addToUFM set x x)
+    | Mk_UniqSet set, x => Mk_UniqSet (UniqFM.addToUFM set x x)
     end.
 
 Definition addListToUniqSet {a} `{Unique.Uniquable a}
@@ -92,45 +82,45 @@ Definition delListFromUniqSet {a} `{Unique.Uniquable a}
    : UniqSet a -> list a -> UniqSet a :=
   fun arg_0__ arg_1__ =>
     match arg_0__, arg_1__ with
-    | UniqSet s, l => UniqSet (UniqFM.delListFromUFM s l)
+    | Mk_UniqSet s, l => Mk_UniqSet (UniqFM.delListFromUFM s l)
     end.
 
 Definition delListFromUniqSet_Directly {a}
    : UniqSet a -> list Unique.Unique -> UniqSet a :=
   fun arg_0__ arg_1__ =>
     match arg_0__, arg_1__ with
-    | UniqSet s, l => UniqSet (UniqFM.delListFromUFM_Directly s l)
+    | Mk_UniqSet s, l => Mk_UniqSet (UniqFM.delListFromUFM_Directly s l)
     end.
 
 Definition delOneFromUniqSet {a} `{Unique.Uniquable a}
    : UniqSet a -> a -> UniqSet a :=
   fun arg_0__ arg_1__ =>
     match arg_0__, arg_1__ with
-    | UniqSet s, a => UniqSet (UniqFM.delFromUFM s a)
+    | Mk_UniqSet s, a => Mk_UniqSet (UniqFM.delFromUFM s a)
     end.
 
 Definition delOneFromUniqSet_Directly {a}
    : UniqSet a -> Unique.Unique -> UniqSet a :=
   fun arg_0__ arg_1__ =>
     match arg_0__, arg_1__ with
-    | UniqSet s, u => UniqSet (UniqFM.delFromUFM_Directly s u)
+    | Mk_UniqSet s, u => Mk_UniqSet (UniqFM.delFromUFM_Directly s u)
     end.
 
 Definition elemUniqSet_Directly {a} : Unique.Unique -> UniqSet a -> bool :=
   fun arg_0__ arg_1__ =>
     match arg_0__, arg_1__ with
-    | a, UniqSet s => UniqFM.elemUFM_Directly a s
+    | a, Mk_UniqSet s => UniqFM.elemUFM_Directly a s
     end.
 
 Definition elementOfUniqSet {a} `{Unique.Uniquable a}
    : a -> UniqSet a -> bool :=
   fun arg_0__ arg_1__ =>
     match arg_0__, arg_1__ with
-    | a, UniqSet s => UniqFM.elemUFM a s
+    | a, Mk_UniqSet s => UniqFM.elemUFM a s
     end.
 
 Definition emptyUniqSet {a} : UniqSet a :=
-  UniqSet UniqFM.emptyUFM.
+  Mk_UniqSet UniqFM.emptyUFM.
 
 Definition mkUniqSet {a} `{Unique.Uniquable a} : list a -> UniqSet a :=
   Data.Foldable.foldl' addOneToUniqSet emptyUniqSet.
@@ -138,14 +128,14 @@ Definition mkUniqSet {a} `{Unique.Uniquable a} : list a -> UniqSet a :=
 Definition filterUniqSet {a} : (a -> bool) -> UniqSet a -> UniqSet a :=
   fun arg_0__ arg_1__ =>
     match arg_0__, arg_1__ with
-    | p, UniqSet s => UniqSet (UniqFM.filterUFM p s)
+    | p, Mk_UniqSet s => Mk_UniqSet (UniqFM.filterUFM p s)
     end.
 
 Definition filterUniqSet_Directly {elt}
    : (Unique.Unique -> elt -> bool) -> UniqSet elt -> UniqSet elt :=
   fun arg_0__ arg_1__ =>
     match arg_0__, arg_1__ with
-    | f, UniqSet s => UniqSet (UniqFM.filterUFM_Directly f s)
+    | f, Mk_UniqSet s => Mk_UniqSet (UniqFM.filterUFM_Directly f s)
     end.
 
 Definition getUniqSet {a} : UniqSet a -> UniqFM.UniqFM a :=
@@ -154,30 +144,30 @@ Definition getUniqSet {a} : UniqSet a -> UniqFM.UniqFM a :=
 Definition intersectUniqSets {a} : UniqSet a -> UniqSet a -> UniqSet a :=
   fun arg_0__ arg_1__ =>
     match arg_0__, arg_1__ with
-    | UniqSet s, UniqSet t => UniqSet (UniqFM.intersectUFM s t)
+    | Mk_UniqSet s, Mk_UniqSet t => Mk_UniqSet (UniqFM.intersectUFM s t)
     end.
 
 Definition isEmptyUniqSet {a} : UniqSet a -> bool :=
-  fun arg_0__ => let 'UniqSet s := arg_0__ in UniqFM.isNullUFM s.
+  fun arg_0__ => let 'Mk_UniqSet s := arg_0__ in UniqFM.isNullUFM s.
 
 Definition lookupUniqSet {a} {b} `{Unique.Uniquable a}
    : UniqSet b -> a -> option b :=
   fun arg_0__ arg_1__ =>
     match arg_0__, arg_1__ with
-    | UniqSet s, k => UniqFM.lookupUFM s k
+    | Mk_UniqSet s, k => UniqFM.lookupUFM s k
     end.
 
 Definition lookupUniqSet_Directly {a}
    : UniqSet a -> Unique.Unique -> option a :=
   fun arg_0__ arg_1__ =>
     match arg_0__, arg_1__ with
-    | UniqSet s, k => UniqFM.lookupUFM_Directly s k
+    | Mk_UniqSet s, k => UniqFM.lookupUFM_Directly s k
     end.
 
 Definition minusUniqSet {a} : UniqSet a -> UniqSet a -> UniqSet a :=
   fun arg_0__ arg_1__ =>
     match arg_0__, arg_1__ with
-    | UniqSet s, UniqSet t => UniqSet (UniqFM.minusUFM s t)
+    | Mk_UniqSet s, Mk_UniqSet t => Mk_UniqSet (UniqFM.minusUFM s t)
     end.
 
 Definition nonDetEltsUniqSet {elt} : UniqSet elt -> list elt :=
@@ -191,14 +181,14 @@ Definition nonDetFoldUniqSet {elt} {a}
    : (elt -> a -> a) -> a -> UniqSet elt -> a :=
   fun arg_0__ arg_1__ arg_2__ =>
     match arg_0__, arg_1__, arg_2__ with
-    | c, n, UniqSet s => UniqFM.nonDetFoldUFM c n s
+    | c, n, Mk_UniqSet s => UniqFM.nonDetFoldUFM c n s
     end.
 
 Definition nonDetFoldUniqSet_Directly {elt} {a}
    : (Unique.Unique -> elt -> a -> a) -> a -> UniqSet elt -> a :=
   fun arg_0__ arg_1__ arg_2__ =>
     match arg_0__, arg_1__, arg_2__ with
-    | f, n, UniqSet s => UniqFM.nonDetFoldUFM_Directly f n s
+    | f, n, Mk_UniqSet s => UniqFM.nonDetFoldUFM_Directly f n s
     end.
 
 Definition nonDetKeysUniqSet {elt} : UniqSet elt -> list Unique.Unique :=
@@ -208,30 +198,23 @@ Definition partitionUniqSet {a}
    : (a -> bool) -> UniqSet a -> (UniqSet a * UniqSet a)%type :=
   fun arg_0__ arg_1__ =>
     match arg_0__, arg_1__ with
-    | p, UniqSet s => GHC.Prim.coerce (UniqFM.partitionUFM p s)
-    end.
-
-Definition pprUniqSet {a}
-   : (a -> GHC.Base.String) -> UniqSet a -> GHC.Base.String :=
-  fun arg_0__ arg_1__ =>
-    match arg_0__, arg_1__ with
-    | f, UniqSet s => UniqFM.pprUniqFM f s
+    | p, Mk_UniqSet s => GHC.Prim.coerce (UniqFM.partitionUFM p s)
     end.
 
 Definition restrictUniqSetToUFM {a} {b}
    : UniqSet a -> UniqFM.UniqFM b -> UniqSet a :=
   fun arg_0__ arg_1__ =>
     match arg_0__, arg_1__ with
-    | UniqSet s, m => UniqSet (UniqFM.intersectUFM s m)
+    | Mk_UniqSet s, m => Mk_UniqSet (UniqFM.intersectUFM s m)
     end.
 
 Definition sizeUniqSet {a} : UniqSet a -> GHC.Num.Int :=
-  fun arg_0__ => let 'UniqSet s := arg_0__ in UniqFM.sizeUFM s.
+  fun arg_0__ => let 'Mk_UniqSet s := arg_0__ in UniqFM.sizeUFM s.
 
 Definition unionUniqSets {a} : UniqSet a -> UniqSet a -> UniqSet a :=
   fun arg_0__ arg_1__ =>
     match arg_0__, arg_1__ with
-    | UniqSet s, UniqSet t => UniqSet (UniqFM.plusUFM s t)
+    | Mk_UniqSet s, Mk_UniqSet t => Mk_UniqSet (UniqFM.plusUFM s t)
     end.
 
 Definition unionManyUniqSets {a} (xs : list (UniqSet a)) : UniqSet a :=
@@ -243,39 +226,39 @@ Definition unionManyUniqSets {a} (xs : list (UniqSet a)) : UniqSet a :=
 Definition uniqSetAll {a} : (a -> bool) -> UniqSet a -> bool :=
   fun arg_0__ arg_1__ =>
     match arg_0__, arg_1__ with
-    | p, UniqSet s => UniqFM.allUFM p s
+    | p, Mk_UniqSet s => UniqFM.allUFM p s
     end.
 
 Definition uniqSetAny {a} : (a -> bool) -> UniqSet a -> bool :=
   fun arg_0__ arg_1__ =>
     match arg_0__, arg_1__ with
-    | p, UniqSet s => UniqFM.anyUFM p s
+    | p, Mk_UniqSet s => UniqFM.anyUFM p s
     end.
 
 Definition uniqSetMinusUFM {a} {b}
    : UniqSet a -> UniqFM.UniqFM b -> UniqSet a :=
   fun arg_0__ arg_1__ =>
     match arg_0__, arg_1__ with
-    | UniqSet s, t => UniqSet (UniqFM.minusUFM s t)
+    | Mk_UniqSet s, t => Mk_UniqSet (UniqFM.minusUFM s t)
     end.
 
 Definition unitUniqSet {a} `{Unique.Uniquable a} : a -> UniqSet a :=
-  fun x => UniqSet (UniqFM.unitUFM x x).
+  fun x => Mk_UniqSet (UniqFM.unitUFM x x).
 
 Definition unsafeUFMToUniqSet {a} : UniqFM.UniqFM a -> UniqSet a :=
-  UniqSet.
+  Mk_UniqSet.
 
 (* External variables:
-     bool cons list negb op_zt__ option Data.Foldable.foldl' Data.Foldable.foldr
-     GHC.Base.Eq_ GHC.Base.Monoid GHC.Base.Semigroup GHC.Base.String GHC.Base.map
-     GHC.Base.mappend GHC.Base.mconcat GHC.Base.mempty GHC.Base.op_z2218U__
-     GHC.Base.op_zlzlzgzg__ GHC.Num.Int GHC.Prim.coerce UniqFM.UniqFM UniqFM.addToUFM
-     UniqFM.allUFM UniqFM.anyUFM UniqFM.delFromUFM UniqFM.delFromUFM_Directly
-     UniqFM.delListFromUFM UniqFM.delListFromUFM_Directly UniqFM.elemUFM
-     UniqFM.elemUFM_Directly UniqFM.emptyUFM UniqFM.equalKeysUFM UniqFM.filterUFM
+     bool cons list op_zt__ option Data.Foldable.foldl' Data.Foldable.foldr
+     GHC.Base.Monoid GHC.Base.Semigroup GHC.Base.map GHC.Base.mappend
+     GHC.Base.mconcat GHC.Base.mempty GHC.Base.op_z2218U__ GHC.Base.op_zlzlzgzg__
+     GHC.Num.Int GHC.Prim.Build_Unpeel GHC.Prim.Unpeel GHC.Prim.coerce UniqFM.UniqFM
+     UniqFM.addToUFM UniqFM.allUFM UniqFM.anyUFM UniqFM.delFromUFM
+     UniqFM.delFromUFM_Directly UniqFM.delListFromUFM UniqFM.delListFromUFM_Directly
+     UniqFM.elemUFM UniqFM.elemUFM_Directly UniqFM.emptyUFM UniqFM.filterUFM
      UniqFM.filterUFM_Directly UniqFM.intersectUFM UniqFM.isNullUFM UniqFM.lookupUFM
      UniqFM.lookupUFM_Directly UniqFM.minusUFM UniqFM.nonDetEltsUFM
      UniqFM.nonDetFoldUFM UniqFM.nonDetFoldUFM_Directly UniqFM.nonDetKeysUFM
-     UniqFM.partitionUFM UniqFM.plusUFM UniqFM.pprUniqFM UniqFM.sizeUFM
-     UniqFM.unitUFM Unique.Uniquable Unique.Unique
+     UniqFM.partitionUFM UniqFM.plusUFM UniqFM.sizeUFM UniqFM.unitUFM
+     Unique.Uniquable Unique.Unique
 *)
